done/Iron/Language/SimpleRef/Base.v
@@ -1,6 +1,37 @@
 
 Require Export Iron.Data.List.
 Require Export Iron.Data.Nat.
+Require Export Iron.Norm.List.
 Require Export Iron.Norm.
-Require Export Iron.Tactics.
+Require Export Iron.Tactics.Rip2.
+Require Export Iron.Tactics.Case.
+Require Export Iron.Tactics.Nope.
+Require Export Iron.Tactics.Break.
+Require Export Iron.Tactics.Rewrite.
+Require Export Iron.Tactics.Down.
+Require Export Iron.Tactics.Have.
+Require Export Iron.Tactics.Exists.
+Require Export Iron.Tactics.Short.
+Require Export Iron.Tactics.LibTactics.
 Require Export Coq.Arith.Compare_dec.
+Require Import Coq.Logic.FunctionalExtensionality.
+
+
+Ltac norm
+ := simpl in *; rip;
+    try (first [norm_nat | norm_lists]).
+
+Ltac tburn0 T
+ := norm; eauto using T; nope.
+
+Ltac tburn T
+ := try (solve [ tburn0 T
+               | red; tburn0 T]).
+
+Tactic Notation "burn"
+ := tburn false.
+
+Tactic Notation "burn" "using" tactic(T) 
+ := tburn T.
+
+Ltac have_auto ::= burn.
